SeqDataStream

TestModels/dafny-dependencies/StandardLibrary/src/Streams.dfy
@@ -12,8 +12,8 @@ module {:options "--function-syntax:4"} StandardLibrary.Streams {
 
   trait DataStream extends Enumerator<BoundedInts.bytes> {
 
-    ghost const value: bytes
-
+    ghost const data: BoundedInts.bytes
+    
     ghost predicate Valid() 
       reads this, Repr 
       ensures Valid() ==> this in Repr 
@@ -27,13 +27,13 @@ module {:options "--function-syntax:4"} StandardLibrary.Streams {
     function ContentLength(): (res: Option<uint64>)
       requires Valid()
       reads this, Repr
-      ensures res.Some? ==> res.value as int == |value|
+      ensures res.Some? ==> res.value as int == |data|
 
     ghost predicate CanProduce(history: seq<((), Option<bytes>)>)
       decreases height
     {
       && (forall o <- Enumerated(Outputs(history)) :: 0 < |o|)
-      && ConcatenatedOutputs(history) <= value
+      && ConcatenatedOutputs(history) <= data
     }
 
     lemma {:axiom} ProducesTerminated(history: seq<((), Option<bytes>)>)
@@ -71,12 +71,13 @@ module {:options "--function-syntax:4"} StandardLibrary.Streams {
       requires Rewindable()
       reads this, Repr
       decreases height, 2
-      ensures res as int <= |value|
+      ensures res as int <= |data|
 
     method Seek(newPosition: uint64)
       requires Valid()
       requires Rewindable()
-      requires newPosition as int <= |value|
+      requires newPosition as int <= |data|
+      modifies Repr
       ensures Valid()
       ensures Position() == newPosition
   }
@@ -98,7 +99,8 @@ module {:options "--function-syntax:4"} StandardLibrary.Streams {
       && this in Repr
       && ValidComponent(wrapped)
       && CanProduce(history)
-      && (length.Some? ==> length.value as int == |value|)
+      && |data| <= UINT64_MAX as int
+      && (length.Some? ==> length.value as int == |data|)
     }
 
     lemma {:axiom} ProducesTerminated(history: seq<((), Option<BoundedInts.bytes>)>)
@@ -110,15 +112,16 @@ module {:options "--function-syntax:4"} StandardLibrary.Streams {
       wrapped.Limit()
     }
 
-    constructor(wrapped: Enumerator<BoundedInts.bytes>, length: Option<uint64>, ghost value: BoundedInts.bytes) 
+    constructor(wrapped: Enumerator<BoundedInts.bytes>, length: Option<uint64>, ghost data: BoundedInts.bytes) 
       requires wrapped.Valid()
       requires wrapped.history == []
-      requires length.Some? ==> length.value as int == |value|
+      requires |data| <= UINT64_MAX as int
+      requires length.Some? ==> length.value as int == |data|
       ensures Valid()
     {
       this.wrapped := wrapped;
       this.length := length;
-      this.value := value;
+      this.data := data;
 
       this.history := [];
       this.Repr := {this} + wrapped.Repr;
@@ -128,7 +131,7 @@ module {:options "--function-syntax:4"} StandardLibrary.Streams {
     function ContentLength(): (res: Option<uint64>)
       requires Valid()
       reads this, Repr
-      ensures res.Some? ==> res.value as int == |value|
+      ensures res.Some? ==> res.value as int == |data|
     {
       length
     }
@@ -142,7 +145,7 @@ module {:options "--function-syntax:4"} StandardLibrary.Streams {
     function Position(): (res: uint64)
       requires Rewindable()
       reads this, Repr
-      ensures res as int <= |value|
+      ensures res as int <= |data|
     {
       // Unreachable
       assert false;
@@ -152,7 +155,7 @@ module {:options "--function-syntax:4"} StandardLibrary.Streams {
     method Seek(newPosition: uint64)
       requires Valid()
       requires Rewindable()
-      requires newPosition as int <= |value|
+      requires newPosition as int <= |data|
       ensures Valid()
       ensures Position() == newPosition
     {
@@ -176,5 +179,112 @@ module {:options "--function-syntax:4"} StandardLibrary.Streams {
     }
   }
 
+  /*
+   * Rewindable stream of a sequence with a configured chunk size.
+   */
+  class SeqDataStream<bytes> extends DataStream {
 
+    const s: BoundedInts.bytes
+    const chunkSize: uint64
+    var position: uint64
+
+    ghost predicate Valid() 
+      reads this, Repr 
+      ensures Valid() ==> this in Repr 
+      ensures Valid() ==> CanProduce(history)
+      decreases height, 0
+    {
+      && this in Repr
+      && CanProduce(history)
+      && s == data
+      && |s| <= UINT64_MAX as int
+      && position as int <= |s|
+      && ConcatenatedOutputs(history) == s[..position]
+      && 0 < chunkSize
+    }
+
+    lemma {:axiom} ProducesTerminated(history: seq<((), Option<BoundedInts.bytes>)>)
+      requires Action().CanProduce(history) 
+      requires (forall i <- Inputs(history) :: i == FixedInput())
+      ensures exists n: nat | n <= Limit() :: Terminated(Outputs(history), StopFn(), n)
+
+    ghost function Limit(): nat {
+      |s|
+    }
+
+    constructor(s: BoundedInts.bytes, chunkSize: uint64)
+      requires |s| <= UINT64_MAX as int
+      requires 0 < chunkSize
+      ensures Valid()
+    {
+      this.data := s;
+      this.s := s;
+      this.position := 0;
+      this.chunkSize := chunkSize;
+
+      this.history := [];
+      this.Repr := {this};
+      this.height := 1;
+    }
+
+    function ContentLength(): (res: Option<uint64>)
+      requires Valid()
+      reads this, Repr
+      ensures res.Some? ==> res.value as int == |data|
+    {
+      Some(|s| as uint64)
+    }
+
+    predicate Rewindable()
+      decreases height, 1
+    {
+      true
+    }
+
+    function Position(): (res: uint64)
+      requires Valid()
+      requires Rewindable()
+      reads this, Repr
+      decreases height, 2
+      ensures res as int <= |data|
+    {
+      position
+    }
+
+    method Seek(newPosition: uint64)
+      requires Valid()
+      requires Rewindable()
+      requires newPosition as int <= |data|
+      modifies Repr
+      ensures Valid()
+      ensures Position() == newPosition
+    {
+      position := newPosition;
+      history := [((), Some(s[..position]))];
+      // TODO: work to do
+      assume {:axiom} Valid();
+    }
+
+    method Invoke(t: ()) returns (r: Option<BoundedInts.bytes>) 
+      requires Requires(t)
+      modifies Modifies(t)
+      decreases Decreases(t).Ordinal()
+      ensures Ensures(t, r)
+    {
+      assume {:axiom} Valid();
+      if position == |s| as uint64 {
+        r := None;
+      } else {
+        // Warning: unbounded integers
+        var size := Math.Min(chunkSize as int, |s| - position as int) as uint64;
+        var newPosition := position + size;
+        r := Some(s[position..newPosition]);
+        position := newPosition;
+      }
+      Update(t, r);
+
+      // TODO: Work to do
+      assume {:axiom} Ensures(t, r);
+    }
+  }
 }
